\documentclass{article}
\usepackage[utf8]{inputenc}

\title{the1}
\author{Halide Yılmaz \\ 2376150}
\date{6 November 2020}
\usepackage[framemethod=TikZ]{mdframed}
\usepackage{natbib}
\usepackage{graphicx}

\begin{document}

\maketitle

\section{Q1}
\subsection{}
\begin{tabular}{|l|c|c|c|c|c|c|}
    \hline
     p & q & $ \neg p $ & $\neg q $ & $ q\rightarrow \neg p $ & $ p \leftrightarrow \neg q $ & $ (q\rightarrow \neg p)   \leftrightarrow (p \leftrightarrow \neg q ) $ \\
    \hline \hline
    T&T&F&F&F&F&T \\
    \hline
    T&F&F&T&T&T&T \\
    \hline
    F&T&T&F&T&T&T\\
    \hline
    F&F&T&T&T&F&F\\ \hline
\end{tabular}
\subsection{}
\begin{tabular}{|c|c|c|c|c|c|c|c|}
     \hline 
     p&q&r&$ p\lor q $&$ r \rightarrow p $&$ r \rightarrow q $&$ (p\lor q )\land (r \rightarrow p) \land  (r \rightarrow q) $&$ [(p\lor q )\land (r \rightarrow p) \land  (r \rightarrow q) ]\rightarrow r$\\ 
     \hline \hline \cr
     T&T&T&T&T&T&T&T\\
     \hline 
     T&T&F&T&T&T&T&F\\
     \hline
     T&F&T&T&T&F&F&T\\
     \hline
     T&F&F&T&T&T&T&F\\
     \hline
     F&T&T&T&F&T&F&T\\
     \hline
     F&T&F&T&T&T&T&F\\
     \hline
     F&F&T&F&F&F&F&T\\
     \hline
     F&F&F&F&T&T&F&T\\
     \hline
\end{tabular}

The conditional statement is not a tautology.
\section{Q2}
\begin{itemize}
    \item $ (p \rightarrow q) \land (p \rightarrow r) \equiv p\rightarrow (q \land r) \quad \Longrightarrow Table7 \quad equation7$
    \item $ \neg (q \land r) \equiv (\neg q \lor \neg r) \quad \Longrightarrow $ De \quad Morgan’s \quad laws 
    \item $ p\rightarrow (q \land r) \equiv \neg (q \land r) \rightarrow \neg p \quad \Longrightarrow $ Table7\quad equation2 (Contrapositive) 
    \item $ \neg (q \land r) \rightarrow \neg p \equiv (\neg q \lor \neg r) \rightarrow \neg p $ 
\end{itemize}
\section{Q3}

\section{Q4}
\subsection{a)}
\begin{mdframed}[]
1: $p \rightarrow q$ \quad\quad\quad\quad\quad PREMİSE \\
2: $r \rightarrow s$ \quad\quad\quad\quad\quad PREMİSE \\
\begin{mdframed}[]
3: q \quad \quad \quad\quad\quad\quad\quad ASSUMPTION \\
\begin{mdframed}[]
4: r\quad\quad\quad\quad\quad\quad\quad ASSUMPTION\\
5: p \quad \quad\quad\quad\quad\quad\quad 1,3, $\rightarrow e\\
6: s  \quad \quad\quad\quad\quad\quad\quad 2,4, \rightarrow e$\\
7: $p \lor r$ \quad\quad\quad\quad\quad\quad 5,$ \lor  i$\\
\end{mdframed}
8: $ s\lor q $ \quad\quad 6,$ \lor $i\\ 
\end{mdframed}
9: $(p\lor r) \rightarrow (s\lor q) $ \quad 7,8, $\rightarrow i$
\end{mdframed}
\newpage
\subsection{b)}
\begin{mdframed}[]
1: $ p\rightarrow (r \rightarrow \neg q)$ \quad \quad ASSUMPTION\\
\begin{mdframed}
2: $ p \land q  \quad \quad ASSUMPTION $\\
3: p \quad \quad 2, $\land e$\\
4: $r\rightarrow \neg q \quad 1,3, \rightarrow e$\\
\begin{mdframed}[]
5: r \quad ASSUMPTION\\
6:$ \neg q \quad 4,5,\rightarrow e$ \\
7: $q \quad 2, \land e$\\
8:$ \bot \quad \quad 6,7,\neg e$\\
\end{mdframed}
9: $\neg r \quad \quad  5-8,\neg i $\\
\end{mdframed}
10:$(p \land q)\rightarrow \neg r \quad \quad 2-9, \rightarrow i$\\
\end{mdframed}
11.$ (p\rightarrow (r \rightarrow \neg q))\rightarrow (p \land q)\rightarrow \neg r \quad \quad 1-10, \rightarrow i$

\section{Q5}

\end{document}
